Add the Reader Monad typeclass and implementation

theories/Control/Classes.v
@@ -1,7 +1,7 @@
 Require Import FreeSpec.Control.
 Require Import FreeSpec.WEq.
 
-(** Monad Transformer
+(** * Monad Transformer
 
  *)
 
@@ -27,3 +27,37 @@ Class MonadState
 
 Arguments put [m s _] (_).
 Arguments get [m s _].
+
+Instance monadtransform_state
+         (t: forall (m: Type -> Type) `{Monad m}, Type -> Type)
+        `{MonadTrans t}
+         (s: Type)
+         (m: Type -> Type)
+        `{MonadState m s}
+  : MonadState (t m) s :=
+  { put := fun x => lift (put x)
+  ; get := lift get
+  }.
+
+(** * Reader Monad
+
+ *)
+
+Class MonadReader
+      (m: Type -> Type)
+      (r: Type) :=
+  { monadreader_is_monad :> Monad m
+  ; ask: m r
+  }.
+
+Arguments ask [m r _].
+
+Instance monadtransform_reader
+         (t: forall (m: Type -> Type) `{Monad m}, Type -> Type)
+        `{MonadTrans t}
+         (r: Type)
+         (m: Type -> Type)
+        `{MonadReader m r}
+  : MonadReader (t m) r :=
+  { ask := lift ask
+  }.
