theories/Control/Reader.v
@@ -1,0 +1,175 @@
+Require Import FreeSpec.Control.
+Require Import FreeSpec.Control.Classes.
+Require Import FreeSpec.Control.Identity.
+Require Import FreeSpec.WEq.
+
+Local Open Scope free_weq_scope.
+
+(** * Definition
+
+ *)
+
+Definition ReaderT
+           (r: Type)
+           (m: Type -> Type)
+          `{Monad m}
+           (a: Type)
+  : Type :=
+  r -> m a.
+
+(** * Functor
+
+ *)
+
+Definition reader_map
+           {m: Type -> Type}
+          `{Monad m}
+           {r: Type}
+           (a b: Type)
+           (f: a -> b)
+           (mr: ReaderT r m a)
+  : ReaderT r m b :=
+  fun x
+  => f <$> (mr x).
+
+Instance reader_Functor
+         (m: Type -> Type)
+        `{Monad m}
+         (r: Type)
+  : Functor (ReaderT r m) :=
+  { map := reader_map
+  }.
+Proof.
+  + intros a A x.
+    cbn.
+    intros y.
+    unfold reader_map.
+    exact (functor_identity (x y)).
+  + intros a b c C u v x.
+    cbn.
+    intros y.
+    unfold reader_map.
+    exact (functor_composition_identity u v (x y)).
+Defined.
+
+(** * Applicative
+
+ *)
+
+Definition reader_pure
+           {m: Type -> Type}
+          `{Monad m}
+           {r: Type}
+           (a: Type)
+           (x: a)
+  : ReaderT r m a :=
+  fun _
+  => pure x.
+
+Definition reader_apply
+           {m: Type -> Type}
+          `{Monad m}
+           {r: Type}
+           (a b: Type)
+           (f: ReaderT r m (a -> b))
+           (x: ReaderT r m a)
+  : ReaderT r m b :=
+  fun r
+  => (f r) <*> (x r).
+
+Instance reader_Applicative
+         (m: Type -> Type)
+        `{Monad m}
+         (r: Type)
+  : Applicative (ReaderT r m) :=
+  { pure := reader_pure
+  ; apply := reader_apply
+  }.
+Proof.
+  + intros a A x.
+    cbn.
+    intros y.
+    unfold reader_apply.
+    exact (applicative_identity (x y)).
+  + intros a b c C u v w.
+    cbn.
+    intros y.
+    unfold reader_apply, reader_pure.
+    exact (applicative_composition (u y) (v y) (w y)).
+  + intros a b B v x.
+    cbn.
+    intros y.
+    unfold reader_apply, reader_pure.
+    exact (applicative_homomorphism v x).
+  + intros a b B u y.
+    cbn.
+    intros z.
+    unfold reader_apply, reader_pure.
+    exact (applicative_interchange (u z) y).
+Defined.
+
+(** * Monad
+
+ *)
+
+Definition reader_bind
+           {m: Type -> Type}
+          `{Monad m}
+           {r: Type}
+           (a b: Type)
+           (p: ReaderT r m a)
+           (f: a -> ReaderT r m b)
+  : ReaderT r m b :=
+  fun x
+  => p x >>= fun y => f y x.
+
+Instance reader_Monad
+         (m: Type -> Type)
+        `{Monad m}
+         (r: Type)
+  : Monad (ReaderT r m) :=
+  { bind := reader_bind
+  }.
+Proof.
+  + intros a b B x f.
+    cbn.
+    intros y.
+    unfold reader_bind, reader_pure.
+    exact (monad_left_identity x _).
+  + intros a A x.
+    cbn.
+    unfold reader_bind, reader_pure.
+    intros y.
+    exact (monad_right_identity (x y)).
+  + intros a b c C f g h.
+    cbn.
+    unfold reader_bind, reader_pure.
+    intros x.
+    exact (monad_bind_associativity (f x) _ _).
+  + intros a b B x f f' Heq.
+    cbn.
+    unfold reader_bind, reader_pure.
+    intros y.
+    apply monad_bind_morphism.
+    intros z.
+    apply Heq.
+Defined.
+
+(** * Reader Monad
+
+ *)
+
+Instance reader_MonadReader
+         (m: Type -> Type)
+        `{Monad m}
+         (r: Type)
+  : MonadReader (ReaderT r m) r :=
+  { ask := fun x
+           => pure x
+  }.
+
+(** * Pure Reader
+
+ *)
+
+Definition Reader r x := ReaderT r Identity x.
